examples/refinement/HighComp.fst
@@ -6,22 +6,22 @@ module U32 = FStar.UInt32
 
 type mint = U32.t
 type state = mint * mint
-//type state = int
 
 // High-level specs live in [comp]
 let comp a = state -> M (a * state)
 
-type hwp 'a = state -> ('a * state -> Type) -> Type
-
-// x:hwp a { monotonic x } 
+type hwp 'a = state -> ('a * state -> Type) -> Type  // x:hwp a { monotonic x } 
 
 // [comp] type with wp
 type comp_wp 'a (wp : hwp 'a) = s0:state -> PURE ('a * state) (wp s0)
 
 type comp_wp' 'a (wp : hwp 'a) = s0:state -> PURE ('a * state) (wp s0)
 
+// [comp] type with preconditions
 let comp_p (a:Type) (pre : state -> Type) (post : state -> a * state -> Type) : GTot Type  =
     s0:state -> Pure (a * state) (pre s0) (post s0)
+
+// WPs 
 
 // can I get these for free?
 unfold
@@ -31,6 +31,8 @@ unfold
 let bind_wp (wp1 : state -> ('a * state -> Type) -> Type)
             (wp2 : 'a -> state -> ('b * state -> Type) -> Type) : state -> ('b * state -> Type) -> Type =
             fun s0 post -> wp1 s0 (function (x, s1) -> wp2 x s1 post)
+
+// Pre and postconditions
 
 unfold
 let trivial_pre = fun s0 -> True
@@ -44,7 +46,7 @@ let bind_pre (#a : Type) (x : a) = fun s0 r -> let (x1, s1) = r in x1 = x /\ s0 
 unfold
 let bind_post (#a : Type) (x : a) = fun s0 r -> let (x1, s1) = r in x1 = x /\ s0 = s1
 
-
+// High-level DSL
 
 val hreturn : (a:Type) -> a -> comp a
 let hreturn (a:Type) (x : a) = fun s -> (x, s)
@@ -52,28 +54,22 @@ let hreturn (a:Type) (x : a) = fun s -> (x, s)
 val hreturn' : (#a:Type) -> (x:a) -> comp_wp a (return_wp x)
 let hreturn' (#a:Type) (x : a) = fun s -> (x, s)
 
+
 val hbind : (a:Type) -> (b:Type) -> comp a -> (a -> comp b) -> comp b
 let hbind (a:Type) (b:Type) (m : comp a) (f : a -> comp b) =
     fun s -> let (x, s1) = m s in f x s1
 
-let hbind' (#a:Type) (#b:Type) (#wp1:hwp a) (#wp2:a -> hwp b) (m : comp_wp a wp1) (f : (x:a) -> comp_wp b (wp2 x)) :
+let hbind' (#a:Type) (#b:Type) (#wp1:hwp a) (#wp2:a -> hwp b) 
+  (m : comp_wp a wp1) (f : (x:a) -> comp_wp b (wp2 x)) :
   comp_wp b (bind_wp wp1 wp2) =
-  fun s ->
-    admit (); 
-    let (a, s1) = m s in
-    f a s1
+  fun s -> admit (); 
+        let (a, s1) = m s in f a s1
+
 
 val hread : i:int -> comp mint
 let hread (i:int) : comp mint =
     fun s -> if i = 0 then (fst s, s)
           else (snd s, s)
-
-val hwrite : i:int -> v:mint -> comp unit
-let hwrite (i:int) (v:mint) : comp unit =
-    fun s -> if i = 0 then ((), (v, snd s))
-          else ((), (fst s, v))
-
-let write_wp (i:nat) (v:mint) : hwp unit = fun s0 post -> post (hwrite i v s0)
 
 let read_wp (i:nat) : hwp mint = fun s0 post -> post (hread i s0)
 
@@ -82,10 +78,19 @@ let hread' (i:nat) : comp_wp mint (read_wp i) =
     fun s -> if i = 0 then (fst s, s)
           else (snd s, s)
 
+
+val hwrite : i:int -> v:mint -> comp unit
+let hwrite (i:int) (v:mint) : comp unit =
+    fun s -> if i = 0 then ((), (v, snd s))
+          else ((), (fst s, v))
+
+let write_wp (i:nat) (v:mint) : hwp unit = fun s0 post -> post (hwrite i v s0)
+
 val hwrite' : i:nat -> v:mint -> comp_wp unit (write_wp i v)
 let hwrite' (i:nat) (v:mint) : comp_wp unit (write_wp i v) =
     fun s -> if i = 0 then ((), (v, snd s))
           else ((), (fst s, v))
+
 
 // NOTE : ommiting type annotations from hread and hwrite defs
 // makes the effect definition fail
